src/principia/mylist/sorting.lean
@@ -1,0 +1,361 @@
+import .mylist
+import ..mynat.nat_sub
+
+-- Sorting algorithms on lists of naturals
+-- can probably be generalised to some type class thing
+
+-- TODO: encode/state criterion for a sorting algorithm to
+-- be stable, and prove it
+-- more algorithms, obviously
+
+namespace hidden
+
+open mynat
+
+universe u
+variable {T: Sort u}
+variables {a b c d m n k x y z: mynat}
+variables {lst lst1 lst2 lst3 xs ys zs: mylist mynat}
+
+def is_sorted (lst: mylist mynat): Prop :=
+∀ a b: mynat,
+  ∀ hbl: b < len lst,
+    ∀ hab: a < b,
+      get a lst (lt_trans hab hbl) ≤
+        get b lst hbl
+
+def count [decidable_eq T]: T → mylist T → mynat
+| _ []        := 0
+| x (y :: ys) := if x = y then
+                 succ (count x ys) else
+                 count x ys
+
+-- this seems more straightforward than using bijections or something.
+-- correct me if I'm wrong
+def is_perm (lst1 lst2: mylist mynat) :=
+∀ m: mynat,
+  count m lst1 = count m lst2
+
+def sort_alg_correct (alg: mylist mynat → mylist mynat) :=
+∀ lst: mylist mynat,
+  is_sorted (alg lst) ∧ is_perm lst (alg lst)
+
+private theorem succ_lt_impl_lt: succ a < n → a < n :=
+@lt_cancel_strong a n 1
+
+theorem adjacent_sorted_implies_sorted:
+(∀ a,
+  ∀ hsal: succ a < len lst,
+    get a lst (succ_lt_impl_lt hsal) ≤
+    get (succ a) lst hsal)
+→ is_sorted lst :=
+begin
+  assume hadj,
+  intros a b hbl hab,
+  rw lt_iff_succ_le at hab,
+  cases hab with d hd,
+  induction d with d d_ih generalizing b, {
+    conv in b {rw hd},
+    simp,
+    apply hadj,
+  }, {
+    conv in b {rw hd},
+    conv in (succ a + succ d) {rw add_succ},
+    have := d_ih _ _ _ rfl,
+    apply le_trans this (hadj _ _),
+    rw lt_iff_succ_le,
+    from le_to_add,
+  },
+end
+
+theorem empty_sorted: is_sorted [] :=
+begin
+  intros a b,
+  assume hbl hab,
+  exfalso,
+  from lt_nzero hbl,
+end
+
+theorem singleton_sorted: is_sorted [x] :=
+begin
+  intros a b,
+  assume hbl hab,
+  exfalso,
+  dsimp [len] at hbl,
+  rw ←one_eq_succ_zero at hbl,
+  rw ←le_iff_lt_succ at hbl,
+  rw le_zero hbl at hab,
+  from lt_nzero hab,
+end
+
+theorem cons_sorted:
+x ≤ y → is_sorted (y :: ys) → is_sorted (x :: y :: ys) :=
+begin
+  assume hxy hstd_yys,
+  apply adjacent_sorted_implies_sorted,
+  intro m,
+  assume hsal,
+  cases m, {
+    from hxy,
+  }, {
+    have hsm := lt_succ_cancel hsal,
+    have hmsm := @lt_to_add_succ m 0,
+    have := hstd_yys m (succ m) hsm hmsm,
+    from this,
+  },
+end
+
+theorem duo_sorted: x ≤ y → is_sorted (x :: y :: []) :=
+(λ h, cons_sorted h singleton_sorted)
+
+theorem tail_sorted: is_sorted (x :: xs) → is_sorted xs :=
+begin
+  assume hstd_xxs,
+  intros a b,
+  assume hbl hab,
+  have := hstd_xxs (succ a) (succ b)
+                   (@lt_add _ _ 1 hbl)
+                   (@lt_add _ _ 1 hab),
+  from this, -- too lazy to change indentation
+end
+
+theorem empty_perm: is_perm [] [] :=
+begin
+  intro m,
+  refl,
+end
+
+theorem singleton_perm: is_perm [x] [x] :=
+begin
+  intro m,
+  refl,
+end
+
+theorem perm_refl: is_perm lst lst :=
+begin
+  intro m,
+  refl,
+end
+
+theorem perm_symm:
+is_perm lst1 lst2 → is_perm lst2 lst1 :=
+begin
+  assume hp12,
+  intro m,
+  symmetry,
+  from hp12 m,
+end
+
+theorem cons_perm:
+is_perm xs ys → is_perm (x :: xs) (x :: ys) :=
+begin
+  assume hpxsys,
+  intro m,
+  dsimp [count],
+  cases (@lem_nat_eq m x) with hmx hmnx, {
+    repeat {rw if_pos hmx},
+    rw hpxsys m,
+  }, {
+    repeat {rw if_neg hmnx},
+    from hpxsys m,
+  },
+end
+
+theorem perm_trans:
+is_perm lst1 lst2 → is_perm lst2 lst3 → is_perm lst1 lst3 :=
+begin
+  assume hp12 hp23,
+  intro m,
+  from eq.trans (hp12 m) (hp23 m),
+end
+
+theorem count_empty: count x [] = 0 := rfl
+
+theorem empty_perm_is_empty:
+is_perm lst [] → lst = [] :=
+begin
+  assume hple,
+  cases lst, {
+    refl,
+  }, {
+    exfalso,
+    have := hple lst_head,
+    dsimp [count] at this,
+    rw if_pos rfl at this,
+    from succ_ne_zero this,
+  },
+end
+
+theorem count_concat:
+count m (lst1 ++ lst2)
+  = count m lst1 + count m lst2 :=
+begin
+  induction lst1 with x xs h_ih, {
+    rw [count_empty, zero_add, empty_concat],
+  }, {
+    dsimp [count],
+    cases (@lem_nat_eq m x) with hmx hmnx, {
+      repeat {rw if_pos hmx},
+      rw h_ih,
+      rw succ_add,
+    }, {
+      repeat {rw if_neg hmnx},
+      from h_ih,
+    },
+  },
+end
+
+theorem perm_concat:
+is_perm xs ys → is_perm lst1 lst2
+  → is_perm (xs ++ lst1) (ys ++ lst2) :=
+begin
+  assume hpxsys hp12,
+  intro m,
+  rw count_concat,
+  rw count_concat,
+  rw hpxsys m,
+  rw hp12 m,
+end
+
+theorem duo_perm:
+is_perm (x :: y :: []) (y :: x :: []) :=
+begin
+  intro m,
+  dsimp [count],
+  cases (@lem_nat_eq m x) with hmx hmnx, {
+    repeat {rw if_pos hmx},
+    cases (@lem_nat_eq m y) with hmy hmny, {
+      repeat {rw if_pos hmy},
+    }, {
+      repeat {rw if_neg hmny},
+      refl,
+    },
+  }, {
+    repeat {rw if_neg hmnx},
+    cases (@lem_nat_eq m y) with hmy hmny, {
+      repeat {rw if_pos hmy},
+      refl,
+    }, {
+      repeat {rw if_neg hmny},
+    },
+  },
+end
+
+-- insertion sort
+
+def insert_aux: mynat → mylist mynat → mylist mynat
+| x []        := [x]
+| x (y :: ys) := if x ≤ y then
+                 x :: y :: ys else
+                 y :: insert_aux x ys
+
+def insertion_sort: mylist mynat → mylist mynat
+| []        := []
+| (x :: xs) := insert_aux x (insertion_sort xs)
+
+-- ew
+theorem insertion_preserves_sorted:
+is_sorted lst → is_sorted (insert_aux x lst) :=
+begin
+  induction lst with y ys h_ih, {
+    assume _,
+    from singleton_sorted,
+  }, {
+    assume h,
+    dsimp [insert_aux],
+    cases le_lem x y with hxy hnxy, {
+      rw if_pos hxy,
+      from cons_sorted hxy h,
+    }, {
+      rw if_neg hnxy,
+      cases hz: insert_aux x ys with z zs, {
+        from singleton_sorted,
+      }, {
+        apply cons_sorted, {
+          cases ys with y' ys, {
+            have: x = z, {
+              dsimp [insert_aux] at hz,
+              from cons_injective_1 hz,
+            },
+            rw ←this,
+            from lt_impl_le hnxy,
+          }, {
+            dsimp [insert_aux] at hz,
+            cases (le_lem x y') with hxy' hnxy', {
+              rw if_pos hxy' at hz,
+              rw ←(cons_injective_1 hz),
+              from lt_impl_le hnxy,
+            }, {
+              rw if_neg hnxy' at hz,
+              rw ←(cons_injective_1 hz),
+              apply h 0 1 _ _, {
+                dsimp [len],
+                apply @lt_add _ _ 1,
+                from zero_lt_succ,
+              }, {
+                from zero_lt_succ,
+              },
+            },
+          },
+        }, {
+          rw ←hz,
+          apply h_ih,
+          from tail_sorted h,
+        },
+      },
+    },
+  },
+end
+
+theorem insertion_sort_is_sorted:
+∀ lst: mylist mynat, is_sorted (insertion_sort lst) :=
+begin
+  intro lst,
+  induction lst with head tail h_ih, {
+    dsimp [insertion_sort],
+    from empty_sorted,
+  }, {
+    dsimp [insertion_sort],
+    from insertion_preserves_sorted h_ih,
+  },
+end
+
+theorem insertion_is_perm:
+is_perm (x :: xs) (insert_aux x xs) :=
+begin
+  induction xs with x' xs h_ih, {
+    from singleton_perm,
+  }, {
+    dsimp [insert_aux],
+    cases (le_lem x x') with hxx' hnxx', {
+      rw if_pos hxx',
+      from perm_refl,
+    }, {
+      rw if_neg hnxx',
+      apply perm_trans _ (cons_perm h_ih),
+      from perm_concat duo_perm perm_refl,
+    },
+  },
+end
+
+theorem insertion_sort_is_perm:
+∀ lst: mylist mynat, is_perm lst (insertion_sort lst) :=
+begin
+  intro lst,
+  induction lst with head tail h_ih, {
+    from empty_perm,
+  }, {
+    dsimp [insertion_sort],
+    have := @cons_perm head _ _ h_ih,
+    from perm_trans this insertion_is_perm,
+  },
+end
+
+theorem insertion_sort_correct:
+sort_alg_correct insertion_sort :=
+(λ lst,
+  and.intro
+    (insertion_sort_is_sorted lst)
+    (insertion_sort_is_perm lst))
+
+end hidden
